theories/Secure/SecurityImpHandler.v
@@ -1,321 +1,48 @@
-From Coq Require Import
-     Arith.PeanoNat
-     Lists.List
-     Strings.String
-     Morphisms
-     Setoid
-     RelationClasses.
-
-From ExtLib Require Import
-     Data.String
-     Structures.Monad
-     Structures.Traversable
-     Data.List.
-
 From ITree Require Import
-     ITree
-     ITreeFacts
-     Events.MapDefault
-     Events.State
-     Events.StateFacts
-     Core.Divergence
-     Dijkstra.TracesIT
-     Secure.SecureEqHalt
-     Secure.SecureEqEuttHalt
-     Secure.SecureEqWcompat
-     Secure.SecureEqBind
-     Secure.SecurityImp
-     Secure.StrongBisimProper
+     Secure.SecurityImpExc.SecurityImp.
+
+
+Definition secure (pc l : sensitivity) (c : stmt) : Prop := True.
+
+Definition join (s1 s2 : sensitivity) :=
+  match s1 with
+  | Public => Public
+  | Private => s2 end.
+
+Variant leq_sense : sensitivity -> sensitivity -> Prop :=
+  | ls_pub s : leq_sense Public s
+  | ls_priv : leq_sense Private Private.
+
+Inductive well_typed_expr (Γ : privacy_map) : sensitivity -> expr -> Prop := 
+  | wte_lit n s : well_typed_expr Γ s (Lit n)
+  | wte_var x : well_typed_expr Γ (Γ x) (Var x)
+  | wte_plus e1 s1 e2 s2 : well_typed_expr Γ s1 e1 -> well_typed_expr Γ s2 e2 ->
+                          well_typed_expr Γ (join s1 s2) (Plus e1 e2)
+  | wte_min e1 s1 e2 s2 : well_typed_expr Γ s1 e1 -> well_typed_expr Γ s2 e2 ->
+                          well_typed_expr Γ (join s1 s2) (Minus e1 e2)
+  | wte_mult e1 s1 e2 s2 : well_typed_expr Γ s1 e1 -> well_typed_expr Γ s2 e2 ->
+                          well_typed_expr Γ (join s1 s2) (Mult e1 e2)
+.
+
+Inductive well_typed_stmt (Γ : privacy_map) : sensitivity -> sensitivity -> stmt -> Prop :=
+  | wts_manual pc l c : secure pc l c -> well_typed_stmt Γ pc l c
+  | wts_skip pc l : well_typed_stmt Γ pc l Skip
+  | wts_seq c1 c2 pc l1 l2 : well_typed_stmt Γ pc l1 c1 -> well_typed_stmt Γ pc l2 c2 ->
+                             well_typed_stmt Γ pc (join l1 l2) (Seq c1 c2)
+  | wts_assign x e pc l l' : well_typed_expr Γ l e -> leq_sense (join l pc) (Γ x) ->
+                          well_typed_stmt Γ pc l' (Assign x e)
+  | wts_if e c1 c2 pc l l1 l2 : well_typed_expr Γ l e ->
+      well_typed_stmt Γ (join pc l) l1 c1 -> well_typed_stmt Γ (join pc l) l2 c2 ->
+                              well_typed_stmt Γ pc (join l1 l2) (If e c1 c2)
+  | wts_while e c l : well_typed_expr Γ Public e -> well_typed_stmt Γ Public l c ->
+                      well_typed_stmt Γ Public l (While e c) 
+  | wts_print e l l' pc : well_typed_expr Γ l' e -> leq_sense (join pc l') l ->
+                       well_typed_stmt Γ pc l' (Output l e)
+  | wts_raise l pc : leq_sense pc l -> well_typed_stmt Γ pc l (Raise l) 
+  | wts_try c1 c2 l l' pc : well_typed_stmt Γ pc l' c1 -> well_typed_stmt Γ (join pc l') l c2 ->
+                            well_typed_stmt Γ pc l (TryCatch c1 c2)
 .
 
 
-Import Monads.
-Import MonadNotation.
-Local Open Scope monad_scope.
-Local Open Scope string_scope.
-
-From Paco Require Import paco.
-
-Definition sense_preorder : Preorder := {|
-  L := sensitivity;
-  leq := fun s1 s2 =>
-           match (s1,s2) with
-           | (Private, Public) => False
-           | _ => True end |}.
-
-Definition priv_io (A : Type) (e : IOE A) :=
-  match e with
-  | LabelledPrint s _ => s end.
-
-Definition product_rel {R1 R2 S1 S2} (RR1: R1 -> S1 -> Prop) (RR2 : R2 -> S2 -> Prop) 
-           (p1 : R1 * R2) (p2 : S1 * S2) : Prop :=
-  RR1 (fst p1) (fst p2) /\ RR2 (snd p1) (snd p2). 
-  
-Definition low_map_equiv (priv : privacy_map ) (s1 s2 : map) : Prop :=
-  forall x, priv x = Public -> s1 x = s2 x.
-
-Lemma low_equiv_update_public : forall (x : var) (v : value) (priv_map : privacy_map) (s1 s2 : map),
-        priv_map x = Public ->  low_map_equiv priv_map s1 s2 ->
-        low_map_equiv priv_map (update x v s1) (update x v s2).
-Proof.
-  intros. red in H0. red. intros. unfold update.
-  destruct (x =? x0) eqn : Heq; auto.
-Qed.
-
-Lemma low_equiv_update_private_l : forall (x : var) (v : value) (priv_map : privacy_map) (s1 s2 : map),
-    priv_map x = Private -> low_map_equiv priv_map s1 s2 ->
-    low_map_equiv priv_map (update x v s1) s2.
-Proof.
-  intros. red in H0. red. intros. unfold update.
-  destruct (x =? x0) eqn : Heq; auto.
-  apply eqb_eq in Heq. subst. rewrite H in H1. discriminate.
-Qed.
-
-Lemma low_equiv_update_private_r : forall (x : var) (v : value) (priv_map : privacy_map) (s1 s2 : map),
-    priv_map x = Private -> low_map_equiv priv_map s1 s2 ->
-    low_map_equiv priv_map s1 (update x v s2).
-Proof.
-  intros. red in H0. red. intros. unfold update.
-  destruct (x =? x0) eqn : Heq; auto.
-  apply eqb_eq in Heq. subst. rewrite H in H1. discriminate.
-Qed.
-
-
-Definition low_eqit_secure_impstate  (b1 b2 : bool) (priv : var -> sensitivity) {R1 R2 : Type} (RR : R1 -> R2 -> Prop )
-           (m1 : stateT map (itree IOE) R1) (m2 : stateT map (itree IOE) R2) : Prop :=
-  forall s1 s2, low_map_equiv priv s1 s2 -> eqit_secure sense_preorder priv_io (product_rel (low_map_equiv priv) RR) b1 b2 Public (m1 s1) (m2 s2).
-
-Definition handle_case {E1 E2 : Type -> Type} {M : Type -> Type} (hl : E1 ~> M) (hr : E2 ~> M) : (E1 +' E2) ~> M :=
-  fun _ e => match e with
-          | inl1 el => hl _ el
-          | inr1 er => hr _ er end.
-
-Definition handle_state_io : forall A, (stateE +' IOE) A -> stateT map (itree IOE) A :=
-  fun _ e => match e with
-          | inl1 el => handleState _ el
-          | inr1 er => fun s => r <- ITree.trigger er;; Ret (s, r) end. 
-
-Definition interp_imp {R} (t : itree (stateE +' IOE) R ) : stateT map (itree IOE) R :=
-  interp_state handle_state_io t. 
-
-Hint Unfold interp_imp.
-Hint Unfold handle_state_io.
-Hint Unfold product_rel.
-
-Ltac use_simpobs :=
-  repeat match goal with 
-         | H : TauF _ = observe ?t |- _ => apply simpobs in H 
-         | H : RetF _ = observe ?t |- _ => apply simpobs in H
-         | H : VisF _ _ = observe ?t |- _ => apply simpobs in H
-  end.
-
-Lemma interp_eqit_secure_imp : forall (R1 R2 : Type) (RR : R1 -> R2 -> Prop) (priv_map : privacy_map) 
-                                 (t1 : itree (stateE +' IOE) R1 ) 
-                                 (t2 : itree (stateE +' IOE) R2),
-    eqit_secure sense_preorder (priv_imp priv_map) RR true true Public t1 t2 ->
-    low_eqit_secure_impstate true true priv_map RR (interp_imp t1 )  (interp_imp t2).
-Proof.
-  intros R1 R2 RR priv_map. pcofix CIH. intros t1 t2 Ht s1 s2 Hs.
-  punfold Ht. red in Ht. remember (observe t1) as ot1. remember (observe t2) as ot2.
-  unfold interp_imp.
-  hinduction Ht before r; intros.
-  - use_simpobs.  
-    rewrite Heqot1. rewrite Heqot2. repeat rewrite interp_state_ret.
-    pfold. constructor. auto.
-  - use_simpobs.
-    rewrite Heqot1. rewrite Heqot2. repeat rewrite interp_state_tau.
-    pfold. constructor. right. pclearbot. apply CIH; auto.
-  - use_simpobs. rewrite Heqot1. rewrite interp_state_tau.
-    pfold. constructor; auto. pstep_reverse.
-  - use_simpobs. rewrite Heqot2. rewrite interp_state_tau.
-    pfold. constructor; auto.  pstep_reverse.
-  - pclearbot. use_simpobs.
-    rewrite Heqot1. rewrite Heqot2. repeat rewrite interp_state_vis.
-    destruct e; cbn.
-    + destruct s; cbn.
-      * repeat rewrite bind_ret_l. pfold. constructor. right. cbn. eapply CIH; auto. 
-        cbv in SECCHECK. unfold get. red in Hs. destruct (priv_map x) eqn : Hx; try contradiction.
-        apply Hs in Hx. rewrite Hx. apply H.
-      * repeat rewrite bind_ret_l. pfold. constructor. right. cbv in SECCHECK. cbn.
-        destruct (priv_map x) eqn : Hx; try contradiction.
-        eapply CIH; auto. apply H. apply low_equiv_update_public; auto.
-   + rewrite bind_bind. rewrite bind_bind.  repeat rewrite bind_trigger. destruct i.
-     cbv in SECCHECK. destruct s; try contradiction. pfold. constructor; auto.
-     left. repeat rewrite bind_ret_l. cbn. pfold. constructor. right. apply CIH; auto. apply H.
- - pclearbot. use_simpobs. rewrite Heqot1. rewrite Heqot2.
-   rewrite interp_state_tau. rewrite interp_state_vis. destruct e; try destruct s.
-   + cbn. rewrite bind_ret_l. pfold. cbn. constructor. right. apply CIH; auto. apply H.
-   + cbn. rewrite bind_ret_l. cbn. pfold. constructor. right. apply CIH; auto. apply H.
-     apply low_equiv_update_private_l; auto. cbv in SECCHECK. 
-     destruct (priv_map x); auto; contradiction.
-   + cbn. cbv in SECCHECK. destruct i. destruct s; try contradiction. rewrite bind_bind.
-     rewrite bind_trigger. setoid_rewrite bind_ret_l. pfold. red. cbn. 
-     rewrite itree_eta'. unpriv_ind. cbn. constructor. right. apply CIH; auto.
-     apply H.
- - pclearbot. use_simpobs. rewrite Heqot1. rewrite Heqot2.
-   rewrite interp_state_tau. rewrite interp_state_vis. destruct e; try destruct s.
-   + cbn. rewrite bind_ret_l. pfold. cbn. constructor. right. apply CIH; auto. apply H.
-   + cbn. rewrite bind_ret_l. cbn. pfold. constructor. right. apply CIH; auto. apply H.
-     apply low_equiv_update_private_r; auto. cbv in SECCHECK. 
-     destruct (priv_map x); auto; contradiction.
-   + cbn. cbv in SECCHECK. destruct i. destruct s; try contradiction. rewrite bind_bind.
-     rewrite bind_trigger. setoid_rewrite bind_ret_l. pfold. red. cbn. 
-     rewrite itree_eta' at 1. unpriv_ind. cbn. constructor. right. apply CIH; auto.
-     apply H.
- - use_simpobs. rewrite Heqot1. rewrite Heqot2. pclearbot.
-   rewrite interp_state_vis. destruct e1; try destruct s; destruct e2; try destruct s; try destruct i; cbn;
-   try (repeat rewrite interp_state_vis; cbn; repeat rewrite bind_ret_l; cbn).
-   + pfold. constructor. right. apply CIH; auto. apply H.
-   + pfold. constructor. right. apply CIH; auto. apply H.
-     apply low_equiv_update_private_r; auto. cbv in SECCHECK2. 
-     destruct (priv_map x0); auto; contradiction.
-   + rewrite bind_bind. rewrite bind_trigger.  cbv in SECCHECK2. destruct s; try contradiction.
-     cbn. setoid_rewrite bind_ret_l. pfold. red. cbn. rewrite itree_eta' at 1.
-     unpriv_ind. cbn. constructor. right. apply CIH; auto. apply H.
-   + pfold. constructor. right. apply CIH. apply H.
-     apply low_equiv_update_private_l; auto. cbv in SECCHECK1. 
-     destruct (priv_map x); auto; contradiction.
-   + pfold. constructor. right. apply CIH. apply H.
-     apply low_equiv_update_private_l; auto. cbv in SECCHECK1. 
-     destruct (priv_map x); auto; contradiction.
-     apply low_equiv_update_private_r; auto. cbv in SECCHECK2. 
-     destruct (priv_map x0); auto; contradiction.
-   + rewrite bind_bind. rewrite bind_trigger. cbv in SECCHECK2. destruct s; try contradiction.
-     setoid_rewrite bind_ret_l.
-      pfold. red. cbn. rewrite itree_eta' at 1. unpriv_ind. cbn. constructor.
-      right. apply CIH; try apply H.
-      apply low_equiv_update_private_l; auto. cbv in SECCHECK1. 
-      destruct (priv_map x); auto; contradiction.
-   + rewrite bind_bind. rewrite bind_trigger. cbv in SECCHECK1. destruct s; try contradiction.
-     setoid_rewrite bind_ret_l. pfold. red. cbn. rewrite itree_eta'. unpriv_ind.
-     cbn. constructor. right. apply CIH; auto. apply H.
-   + rewrite bind_bind. rewrite bind_trigger. setoid_rewrite bind_ret_l. pfold. red. cbn.
-     rewrite itree_eta'. unpriv_ind. cbn. constructor. right. apply CIH. apply H.
-     apply low_equiv_update_private_r; auto. cbv in SECCHECK2. 
-     destruct (priv_map x); auto; contradiction.
-   + repeat rewrite bind_bind. repeat rewrite bind_trigger. repeat setoid_rewrite bind_ret_l. 
-     cbn. pfold. red. cbn. destruct i0. unpriv_co.
-     left. pfold. constructor. right. apply CIH; auto. apply H.
- - use_simpobs. rewrite Heqot1. rewrite interp_state_vis.
-   destruct e; try destruct s; cbn.
-   + rewrite bind_ret_l. cbn. pfold. constructor; auto. pstep_reverse.
-   + rewrite bind_ret_l. cbn. pfold. constructor; auto. pstep_reverse. eapply H0; eauto.
-     apply low_equiv_update_private_l; auto. cbv in SECCHECK. 
-     destruct (priv_map x); auto; contradiction.
-   + rewrite bind_bind. rewrite bind_trigger. destruct i. destruct s.
-     cbv in SECCHECK; try contradiction. setoid_rewrite bind_ret_l.
-     cbn. pfold. red. cbn. unpriv_ind. constructor; auto. pstep_reverse.
- - use_simpobs. rewrite Heqot2. rewrite interp_state_vis.
-   destruct e; try destruct s; cbn.
-   + rewrite bind_ret_l. cbn. pfold. constructor; auto. pstep_reverse.
-   + rewrite bind_ret_l. cbn. pfold. constructor; auto. pstep_reverse. eapply H0; eauto.
-     apply low_equiv_update_private_r; auto. cbv in SECCHECK. 
-     destruct (priv_map x); auto; contradiction.
-   + rewrite bind_bind. rewrite bind_trigger. destruct i. destruct s.
-     cbv in SECCHECK; try contradiction. setoid_rewrite bind_ret_l.
-     cbn. pfold. red. cbn. unpriv_ind. constructor; auto. pstep_reverse.
- - destruct e; try destruct s; try destruct i; exfalso; inv SIZECHECK;  apply H0; auto; apply tt.
- -  destruct e; try destruct s; try destruct i; exfalso; inv SIZECHECK;  apply H0; auto; apply tt.
- -  destruct e1; try destruct s; try destruct i; exfalso; inv SIZECHECK;  apply H0; auto; apply tt.
- -  destruct e2; try destruct s; try destruct i; exfalso; inv SIZECHECK;  apply H0; auto; apply tt.
-Qed.
-
-Section GeneralStateHandler.
-
-Context (S : Type).
-Context (RS : S -> S -> Prop).
-
-Context (E1 E2 : Type -> Type).
-
-Context (handler : E1 ~> stateT S (itree E2) ).
-
-Context (Label : Preorder).
-Context (priv1 : forall A, E1 A -> L).
-Context (priv2 : forall A, E2 A -> L).
-Context (l : L).
-
-
-
-Definition state_eqit_secure {R1 R2 : Type} (b1 b2 : bool) (RR : R1 -> R2 -> Prop) 
-           (m1 : stateT S (itree E2) R1) (m2 : stateT S (itree E2) R2) := 
-  forall s1 s2, RS s1 s2 -> eqit_secure Label priv2 (product_rel RS RR) b1 b2 l (m1 s1) (m2 s2).
-  
-Definition top2 {R1 R2} (r1 : R1) (r2 : R2) : Prop := True. 
-
-Variant handler_respects_priv (A : Type) (e : E1 A) : Prop :=
-  | respect_private (SECCHECK : ~ leq (priv1 A e) l ) (RESCHECK : state_eqit_secure true true top2 (handler A e) (handler A e) )
-  | respect_public (SECCHECK : leq (priv1 A e) l ) (RESCHECK : state_eqit_secure true true eq (handler A e) (handler A e)).
-
-Context (Hhandler : forall A (e : E1 A), handler_respects_priv A e).
-
-
-(* I believe that this is a sound reasoning principle,
-   however it looks like the proof could get a little hairy,
-   if I could use gpaco and use the bind and transitivity closures, many of these cases become easy
-   however, this pushes us up against *)
-Lemma interp_eqit_secure_state : forall (R1 R2 : Type) (RR : R1 -> R2 -> Prop) (t1 : itree E1 R1) (t2 : itree E1 R2),
-    eqit_secure Label priv1 RR true true l t1 t2 ->
-    state_eqit_secure true true RR (interp_state handler t1) (interp_state handler t2).
-Proof.
-  intros R1 R2 RR. pcofix CIH. intros t1 t2 Ht s1 s2 Hs. punfold Ht.
-  red in Ht. remember (observe t1) as ot1. remember (observe t2) as ot2.
-  hinduction Ht before r; intros; use_simpobs.
-  - rewrite Heqot1. rewrite Heqot2. repeat rewrite interp_state_ret. pfold. constructor. auto.
-  - rewrite Heqot1. rewrite Heqot2. repeat rewrite interp_state_tau. pfold. constructor. 
-    pclearbot. right. apply CIH; auto.
-  - rewrite Heqot1. rewrite interp_state_tau. pfold. constructor; auto. pstep_reverse.
-  - rewrite Heqot2. rewrite interp_state_tau. pfold. constructor; auto. pstep_reverse.
-  - rewrite Heqot1. rewrite Heqot2. repeat rewrite interp_state_vis.
-    specialize (Hhandler A e). pclearbot. repeat rewrite bind_tau.
-    (* could use the bind closure here, but maybe we can do manually for now*)
-    repeat setoid_rewrite <- interp_state_tau. inv Hhandler; try contradiction.
-    specialize (RESCHECK s1 s2 Hs).
-    (* should hold but will take weird lemma, essentially an application of the bind closure
-       frustratingly this proof could end up being as complicated as the eqit_secure_bind proof *)
-    admit.
-  - pclearbot. rewrite Heqot1. rewrite Heqot2. rewrite interp_state_vis.
-    specialize (Hhandler A e). inv Hhandler; try contradiction.
-    admit.
-  - pclearbot. rewrite Heqot1. rewrite Heqot2. rewrite interp_state_vis.
-    specialize (Hhandler A e). inv Hhandler; try contradiction.
-    admit.
-  - pclearbot. rewrite Heqot1. rewrite Heqot2. repeat rewrite interp_state_vis.
-    specialize (Hhandler _ e1) as He1. specialize (Hhandler _ e2) as He2.
-    inv He1; inv He2; try contradiction. admit.
-  - rewrite Heqot1. rewrite interp_state_vis. specialize (Hhandler _ e).
-    inv Hhandler; try contradiction. (* seems to be a place I need that RS is a PER, can add that assumption *)
-    admit.
-  - rewrite Heqot2. rewrite interp_state_vis. specialize (Hhandler _ e).
-    inv Hhandler; try contradiction. admit.
-  - pclearbot. rewrite Heqot1. rewrite interp_state_vis. rewrite Heqot2.
-    specialize (Hhandler _ e). inv Hhandler; try contradiction. red in RESCHECK.
-    admit.
-  - pclearbot. rewrite Heqot1. rewrite Heqot2. rewrite interp_state_vis.
-    specialize (Hhandler _ e). inv Hhandler; try contradiction. red in RESCHECK.
-    (* this is the different private halt stuff *) admit.
-  - pclearbot. rewrite Heqot1. rewrite Heqot2. repeat rewrite interp_state_vis.
-    (* might basically degenrate to cases from teh bind proof, same with the other empties *)
-    admit.
-  - pclearbot. rewrite Heqot1. rewrite Heqot2. repeat rewrite interp_state_vis.
+Lemma well_typed_stmt_correct : forall Γ pc l c, well_typed_stmt Γ pc l c -> secure pc l c.
 Abort.
-
-End GeneralStateHandler.
-
-
-(* 
-1. Write the paper
-2. Security preserving compiler correctness Imp with IO
-   a. Semantics for Imp +
-   b. Handler security preservation +
-   c. Semantics for Asm +
-   d. Handler security preservation for Asm
-   e. Imp2Asm compiler +'
-   f. Imp2Asm correctness (should not involve coinduction)
-3. General relation of state interpreters and security
-4. Security preserving compiler correctness Imp with IO and private exceptions
-5. Write a type system for Imp and prove soundness
-   a. "Manual" inference rule 
-              |- c1   |= c2
-              -------------- Manual_R
-                |- c1; c2
-*)
