theories/Events/ExceptionFacts.v
@@ -51,6 +51,24 @@ Proof.
       gstep. constructor. gfinal. left. eauto.
 Qed.
 
+Global Instance proper_eutt_try_catch {E Err R} : Proper (eutt eq ==> pointwise_relation Err (eutt eq) ==> eutt eq) (@try_catch Err R E).
+Proof.
+  intros t1 t2 Ht k1 k2 Hk. red in Hk. generalize dependent t2. revert t1.
+  ginit. gcofix CIH. intros. unfold try_catch. do 2 rewrite unfold_iter_ktree.
+  punfold Ht. red in Ht.
+  hinduction Ht before r; intros; subst; eauto; try inv CHECK; pclearbot.
+  - repeat rewrite bind_ret_l. gfinal; right. pfold; constructor; auto.
+  - repeat rewrite bind_ret_l. gstep; constructor. gfinal. left. eauto.
+  - destruct e.
+    + destruct e. cbn. repeat rewrite bind_map. repeat rewrite bind_ret_r.  gfinal.
+      right. eapply paco2_mon; try apply Hk. intros; contradiction.
+    + cbn. repeat rewrite bind_map. repeat rewrite bind_trigger. gstep. constructor. intros.
+      gstep. constructor. gfinal. left. eauto.
+  - rewrite bind_ret_l. rewrite tau_euttge. rewrite unfold_iter_ktree. eapply IHHt; eauto.
+  - rewrite bind_ret_l. rewrite tau_euttge. rewrite unfold_iter_ktree. eapply IHHt; eauto.
+Qed.
+
+
 Global Instance proper_eqitree_throw_prefix {E Err R b} : Proper (eqit eq b b ==> eqit eq b b) (@throw_prefix Err R E).
 Proof.
   intros t1 t2 Ht. generalize dependent t2. revert t1.
