theories/Secure/SecurityImpExc/ITreeForall.v
@@ -1,0 +1,153 @@
+From Coq Require Import
+     Arith.PeanoNat
+     Lists.List
+     Strings.String
+     Morphisms
+     Setoid
+     RelationClasses
+     Logic.Classical_Prop
+.
+
+From ExtLib Require Import
+     Data.String
+     Structures.Monad
+     Structures.Traversable
+     Data.List.
+
+From ITree Require Import
+     ITree
+     ITreeFacts
+     Dijkstra.ITrace (* where ITrace.inj_existT is*)
+.
+
+From Paco Require Import paco.
+
+Import Monads.
+Import MonadNotation.
+Local Open Scope monad_scope.
+Local Open Scope string_scope.
+
+
+Variant itree_forallF (E : Type -> Type) (R : Type) (F : itree E R -> Prop) (PE : forall A : Type, E A -> Prop) (PR : R -> Prop ) : itree' E R -> Prop :=
+  | itree_forall_ret r : PR r -> itree_forallF E R F PE PR (RetF r)
+  | itree_forall_tau t : F t ->  itree_forallF E R F PE PR (TauF t)
+  | itree_forall_vis A (e : E A) k : PE A e -> (forall a : A, F (k a)) -> itree_forallF E R F PE PR (VisF e k)
+.
+
+Hint Constructors itree_forallF.
+
+Definition itree_forall_ E R PE PR F t := itree_forallF E R F PE PR (observe t).
+
+Lemma itree_forall_monot {E R} PE PR : monotone1 (@itree_forall_ E R PE PR).
+Proof.
+  repeat intro. red in IN. red. induction IN; auto.
+Qed.
+
+Hint Resolve itree_forall_monot : paco.
+
+Definition itree_forall {E R} PE PR t := paco1 (itree_forall_ E R PE PR) bot1 t.
+
+Lemma itree_forall_proper_aux: forall (E : Type -> Type) (R : Type) (PE : forall A : Type, E A -> Prop)
+                                  (PR : R -> Prop) (t1 t2 : itree E R),
+    (t1 ≈ t2)%itree -> itree_forall PE PR t1 -> itree_forall PE PR t2.
+Proof.
+  intros E R PE PR. pcofix CIH. intros t1 t2 Heutt Hforall.
+  pfold. red. punfold Hforall. red in Hforall.
+  punfold Heutt. red in Heutt. induction Heutt; subst; auto.
+  - inv Hforall. auto.
+  - inv Hforall. pclearbot. constructor. right. eapply CIH; eauto.
+  - inv Hforall. inj_existT. subst. pclearbot.
+    constructor; auto. intros. right. eapply CIH; eauto. apply H3.
+  - apply IHHeutt. inv Hforall. pclearbot. punfold H0.
+  - constructor. left. pfold. red. apply IHHeutt. auto.
+Qed.
+
+Global Instance itree_forall_proper_eutt {E R PE PR} : Proper (eutt eq ==> iff) (@itree_forall E R PE PR).
+Proof.
+  intros t1 t2 Heutt. split; intros.
+  - eapply itree_forall_proper_aux; eauto.
+  - symmetry in Heutt. eapply itree_forall_proper_aux; eauto.
+Qed.
+
+Variant itree_forall_bind_clo E R PE (PR : R -> Prop)  (r : itree E R -> Prop ) : itree E R -> Prop := 
+  | ifbc_intro S (t : itree E S) (k : S -> itree E R) (Pinv : S -> Prop) :
+      itree_forall PE Pinv t -> (forall s, Pinv s -> r (k s) ) ->
+      itree_forall_bind_clo E R PE PR r (ITree.bind t k)
+.
+
+Lemma itree_forall_bind_clo_wcompat E R PE PR : 
+  wcompatible1 (itree_forall_ E R PE PR) (itree_forall_bind_clo E R PE PR) .
+Proof.
+  constructor.
+  - red. intros. induction IN; eauto. econstructor; eauto.
+  - intros r t Hclo. inv Hclo. red. unfold observe. cbn. punfold H.
+    red in H. inv H.
+    + eapply itree_forall_monot; eauto.
+      intros t Hrt. red. gfinal. eauto.
+    + cbn. constructor. gclo. pclearbot. econstructor; eauto. intros.
+      gfinal. right. pfold. eapply itree_forall_monot; eauto.
+    + cbn. pclearbot. constructor; auto. intros. gclo.
+      econstructor; try apply H3. intros.  gfinal.
+      right. pfold. eapply itree_forall_monot; eauto.
+Qed.
+
+Inductive itree_forall_trans_clo E R (r : itree E R -> Prop)
+  : itree E R -> Prop :=
+| itree_forall_trans_clo_intro t1 t1'
+      (EQV: t1 ≅ t1')
+      (Ht2 : r t1')
+  : itree_forall_trans_clo E R r t1.
+
+Lemma itree_forall_trans_clo_wcompat E R PE PR : 
+  wcompatible1 (itree_forall_ E R PE PR) (itree_forall_trans_clo E R ) .
+Proof.
+  constructor.
+  - red. intros. induction IN; eauto. econstructor; eauto.
+  - intros r t1 Hclo. inv Hclo. red. red in Ht2. punfold EQV.
+    red in EQV. inv EQV; try inv CHECK.
+    + rewrite <- H in Ht2. inv Ht2. constructor; auto.
+    + constructor. pclearbot. rewrite <- H in Ht2. inv Ht2. gclo.
+      econstructor; eauto. gfinal. eauto.
+    + pclearbot. rewrite <- H in Ht2. inv Ht2. ITrace.inj_existT; subst.
+      constructor; auto. intros. gclo. econstructor; eauto. gfinal. eauto.
+Qed.
+
+Hint Resolve itree_forall_trans_clo_wcompat : paco.
+
+Locate geuttgen_cong_eqit_eq.
+
+Instance itree_forall_gpaco_proper {E R PE PR r rg} : Proper (eq_itree eq ==> flip impl) 
+                                                             (gpaco1 (itree_forall_ E R PE PR) (itree_forall_trans_clo E R) r rg).
+Proof.
+  intros t1 t2 Heq H. gclo. econstructor; eauto. 
+Qed.
+
+Lemma itree_forall_clo_bind E R PE PR : 
+  itree_forall_bind_clo E R PE PR <2= gupaco1 (itree_forall_ E R PE PR) (itree_forall_trans_clo E R).
+Proof.
+  intros r t H. generalize dependent t. gcofix CIH. intros t Ht. inv Ht.
+  pinversion H; try apply simpobs in H1.
+  - rewrite H1. rewrite bind_ret_l. gfinal. eauto.
+  - rewrite H1. rewrite bind_tau. gstep. constructor. gfinal. left. eapply CIH.
+    econstructor; eauto.
+  - rewrite H1. rewrite bind_vis. gstep. constructor; auto. intros. gfinal. left. apply CIH.
+    econstructor; eauto. apply H3.
+Qed.
+
+Lemma itree_forall_bind E S R (PE : forall A, E A -> Prop) (PS : S -> Prop) (PR : R -> Prop) t k :
+  itree_forall PE PS t -> (forall s, PS s -> itree_forall PE PR (k s) ) ->
+  itree_forall PE PR (ITree.bind t k).
+Proof.
+  intros. ginit. guclo itree_forall_clo_bind. econstructor; eauto.
+  intros. gfinal. right. apply H0; auto.
+Qed.
+
+Lemma itree_forall_iter_ev (A B : Type) E  (body : A -> itree E (A + B) ) init
+  (PE : forall A, E A -> Prop) : (forall a, itree_forall PE (fun _ => True) (body a) ) -> itree_forall PE (fun _ => True) (iter body init).
+Proof.
+  revert init. ginit. gcofix CIH. intros a Hbody. setoid_rewrite unfold_iter.
+  guclo itree_forall_clo_bind. econstructor. apply Hbody. intros [a' | b] _.
+  - gstep. constructor. gfinal; eauto.
+  - gstep. constructor; auto.
+Qed.
+
