theories/Secure/SecurityImpExc/RaiseException.v
@@ -1,0 +1,277 @@
+From Coq Require Import
+     Arith.PeanoNat
+     Lists.List
+     Strings.String
+     Morphisms
+     Setoid
+     RelationClasses
+     Logic.Classical_Prop
+.
+
+From ExtLib Require Import
+     Data.String
+     Structures.Monad
+     Structures.Traversable
+     Data.List.
+
+From ITree Require Import
+     ITree
+     ITreeFacts
+     Events.MapDefault
+     Events.State
+     Events.StateFacts
+     Events.Exception
+     Events.ExceptionFacts
+     Core.Divergence
+     Dijkstra.TracesIT
+     Dijkstra.ITrace
+     Secure.SecureEqHalt
+     Secure.SecureEqEuttHalt
+     Secure.SecureEqWcompat
+     Secure.SecureEqBind
+     Secure.SecurityImpExc.SecurityImp
+     Secure.SecurityImpExc.SecurityImpHandler
+     Secure.StrongBisimProper
+     Secure.SecurityImpExc.ITreeForall
+.
+
+
+Import Monads.
+Import MonadNotation.
+Local Open Scope monad_scope.
+Local Open Scope string_scope.
+
+From Paco Require Import paco.
+
+Instance sense_preorder_in : Preorder := sense_preorder.
+
+Definition join (s1 s2 : sensitivity) :=
+  match s1 with
+  | Public => s2
+  | Private => Private end.
+
+Ltac case_leq l1 l2 := destruct (classic (@leq sense_preorder l1 l2) ).
+
+Lemma leq_sense_trans (l1 l2 l3 : sensitivity) : leq l1 l2 -> leq l2 l3 -> leq l1 l3.
+Proof.
+  intros. destruct l1; auto.
+  destruct l2; destruct l3; auto.
+Qed.
+
+Lemma leq_sense_join_l (l1 l2 : sensitivity) : leq l1 (join l1 l2).
+Proof.
+  destruct l1; destruct l2; cbn; auto.
+Qed.
+
+Lemma leq_sense_join_r (l1 l2 : sensitivity) : leq l2 (join l1 l2).
+Proof.
+  destruct l1; destruct l2; cbn; auto.
+Qed.
+
+Definition raises_exception {R : Type} (e : impExcE void ) (t : itree (impExcE +' IOE) R) : Prop :=
+  exists (t' : itree (impExcE +' IOE) unit) , can_converge tt t' /\ t ≈ (u <- t';; v <- trigger e;; match v : void with end).
+
+Instance proper_raises_exception {R e} : Proper (eutt eq ==> iff) (@raises_exception R e).
+Proof.
+  repeat intro. unfold raises_exception. setoid_rewrite H. tauto.
+Qed.
+
+Lemma raises_exception_ret e R (r : R) : ~ raises_exception e (Ret r).
+Proof.
+  intro. red in H. destruct H as [t' [_ Ht'] ].
+  cbn in Ht'. setoid_rewrite bind_trigger in Ht'. punfold Ht'. red in Ht'. cbn in *.
+  remember (RetF r) as x. remember  (observe
+             (ITree.bind t'
+                (fun _ : unit =>
+                 Vis (subevent void e)
+                   (fun x : void =>
+                    match x return (itree (impExcE +' IOE) R) with
+                    end)))) as y.
+  hinduction Ht' before r; intros; inv Heqx; inv Heqy; try discriminate.
+  - unfold observe in H0. cbn in H0. destruct (observe t'); try discriminate.
+  - unfold observe in H0. cbn in H0. destruct (observe t'); try discriminate. cbn in H0.
+    injection H0 as H0. apply IHHt' with (t' := t); eauto. subst. auto.
+Qed.
+
+Lemma try_catch_raise_exception {R} (t1 : itree (impExcE +' IOE) R) k2 : 
+  forall e t', can_converge tt t' /\ t1 ≈ (u <- t';; v <- trigger (Throw _ e);; match v : void with end) -> 
+          try_catch t1 k2 ≈ u <- t';; (k2 e).
+Proof.
+  intros e t' [Hconv Heq]. setoid_rewrite Heq. clear Heq.
+  induction Hconv.
+  - rewrite H. setoid_rewrite bind_ret_l. setoid_rewrite bind_trigger.
+    setoid_rewrite try_catch_exc. reflexivity.
+  - rewrite H. setoid_rewrite bind_vis.
+    destruct e0.
+    + destruct e0; contradiction.
+    + setoid_rewrite try_catch_ev. apply eqit_Vis. intros. rewrite tau_eutt.
+      destruct i. destruct u. destruct b. apply IHHconv.
+Qed.
+
+Lemma raises_exception_ev:
+  forall (R : Type) 
+      (k : unit ->
+           itree (impExcE +' IOE) R)
+    (ev : IOE unit),
+    (forall e : impExcE void,
+        ~ raises_exception e (Vis (inr1 ev) k ) ) ->
+
+      forall (e : impExcE void),
+      ~ raises_exception e (k tt).
+Proof.
+   intros. intro Hcontra.
+   red in Hcontra. destruct Hcontra as [t' Ht'].
+   destruct Ht'. apply (H e). red. cbn in *.
+   exists (Vis (inr1 ev) (fun _ => t') ).
+   split.
+   - eapply conv_vis. reflexivity. cbn. apply H0. Unshelve. apply tt.
+   - rewrite bind_vis. apply eqit_Vis. intros []. auto.
+Qed.
+
+Lemma try_catch_not_raise_exception {R} (t1 : itree (impExcE +' IOE) R) k2 :
+  (forall e, ~ raises_exception e t1) -> try_catch t1 k2 ≈ t1.
+Proof.
+  revert t1. unfold try_catch. ginit. gcofix CIH. intros. 
+  setoid_rewrite unfold_iter. destruct (observe t1) eqn : Ht1.
+  - setoid_rewrite Ht1. setoid_rewrite bind_ret_l. symmetry in Ht1. use_simpobs.
+    rewrite Ht1. gfinal. right. pfold; constructor; auto.
+  - setoid_rewrite Ht1. setoid_rewrite bind_ret_l. symmetry in Ht1; use_simpobs.
+    rewrite Ht1. gstep. constructor. gfinal. left. eapply CIH; eauto.
+    assert (t1 ≈ t). rewrite Ht1. apply tau_eutt. setoid_rewrite <- H.
+    auto.
+  - setoid_rewrite Ht1. destruct e.
+    + destruct i. exfalso. clear CIH. symmetry in Ht1. use_simpobs.
+      setoid_rewrite Ht1 in H0. eapply H0 with (e :=  (Throw _ s)  ). red. exists (Ret tt).
+      split; try (constructor; reflexivity; fail).
+      tau_steps. apply eqit_Vis. intros [].
+    + cbn. setoid_rewrite bind_bind. setoid_rewrite bind_trigger.
+      symmetry in Ht1. use_simpobs. rewrite Ht1. gstep. constructor.
+      intros. red. rewrite bind_ret_l. rewrite tau_euttge. gfinal. left. apply CIH.
+      intros. destruct i. destruct v. eapply raises_exception_ev. 
+      setoid_rewrite Ht1 in H0. eauto.
+Qed.
+
+Lemma classic_raise_exception {R} (t : itree (impExcE +' IOE) R) :
+  (forall e, ~ raises_exception e t) \/ (exists e, raises_exception e t).
+Proof.
+  destruct (classic (exists e, raises_exception e t) ); eauto.
+Qed.
+
+Lemma try_catch_ret {R} (t : itree (impExcE +' IOE) R) k :
+  (exists r, can_converge r t) -> try_catch t k ≈ t.
+Proof.
+  intro Hconv. destruct Hconv as [r Hconv].
+  induction Hconv.
+  - rewrite H. rewrite try_catch_ret. reflexivity.
+  - destruct e.
+    + destruct i; contradiction.
+    + destruct i.  destruct b. rewrite H.
+      rewrite try_catch_ev. apply eqit_Vis. intros []. rewrite tau_eutt.
+      auto.
+Qed.
+
+
+Definition can_raise_exception {R} (e : impExcE void ) (m : stateT map (itree (impExcE +' IOE)) R  ) : Prop :=
+  exists s, raises_exception e (m s).
+
+
+Definition max_exception_label {R} l (m: stateT map (itree (impExcE +' IOE)) R)  := forall l', can_raise_exception (Throw _ l') m -> leq l' l.
+
+Lemma seq_max_exception {R1 R2} lexn1 lexn2 (m1 : stateT map (itree (impExcE +' IOE)) R1) (m2 : stateT map (itree (impExcE +' IOE)) R2) :
+  max_exception_label lexn1 m1 -> max_exception_label lexn2 m2 -> max_exception_label (join lexn1 lexn2) (m1 ;; m2).
+Proof.
+  intros Hm1 Hm2. red. intros lmax Hexc. red in Hm1, Hm2.
+  red in Hexc. destruct Hexc as [s Hs]. red in Hs.
+  destruct Hs as [t' [Hconv Ht'] ]. generalize dependent m1. generalize dependent m2.
+  induction Hconv; intros.
+  - rewrite H in Ht'. cbn in Ht'. rewrite bind_ret_l in Ht'. rewrite bind_trigger in Ht'.
+    apply eqit_inv_bind_vis in Ht'.
+    destruct Ht' as [Ht' | Ht'].
+    + destruct Ht' as [kxa [Hkxa _ ] ]. 
+      enough (leq lmax lexn1). eapply leq_sense_trans; eauto. apply leq_sense_join_l.
+      apply Hm1. red. exists s. rewrite Hkxa. red. exists (Ret tt). split.
+      constructor; reflexivity. setoid_rewrite bind_ret_l. setoid_rewrite bind_trigger. apply eqit_Vis.
+      intros [].
+    + destruct Ht' as [ [s1 r1] [Hm1s Hm2s ] ]. cbn in Hm2s.
+      enough (leq lmax lexn2). eapply leq_sense_trans; eauto. apply leq_sense_join_r.
+      apply Hm2. exists s1. exists (Ret tt). split.
+      constructor; reflexivity.
+      setoid_rewrite Hm2s. setoid_rewrite bind_ret_l. setoid_rewrite bind_trigger.
+      apply eqit_Vis. intros [].
+  - destruct e.
+    + destruct i; contradiction.
+    + destruct i. setoid_rewrite H in Ht'. setoid_rewrite bind_vis in Ht'.
+      apply eqit_inv_bind_vis in Ht' as Ht''. destruct Ht'' as [Ht'' | Ht''].
+      * destruct Ht'' as [kxa [Hkxa _ ] ]. eapply IHHconv with (m1 := fun s => kxa tt); eauto.
+        -- intros. apply Hm1. exists s. rewrite Hkxa.
+           red. red in H0. destruct H0 as [ _ Hkxa']. red in Hkxa'.
+           destruct Hkxa' as [t'' [Hconv' Ht''] ].
+           exists (Vis (inr1 (LabelledPrint s0 v)) (fun _ => t'') ). split.
+           { eapply conv_vis. reflexivity. eauto. Unshelve. apply tt. }
+           setoid_rewrite bind_vis. apply eqit_Vis. intros []. auto.
+        -- cbn. cbn in Ht'. rewrite Hkxa in Ht'. rewrite bind_vis in Ht'.  apply eqit_inv_vis in Ht'.
+           destruct Ht'. destruct b. apply H1.
+      * destruct Ht'' as [ [s1 r1] [Hm1s1 Hm2s2] ]. cbn in Hm2s2.
+       enough (leq lmax lexn2). eapply leq_sense_trans; eauto. apply leq_sense_join_r.
+       apply Hm2. exists s1. exists (trigger (LabelledPrint s0 v);; k tt ). split.
+       { eapply conv_vis. unfold trigger. setoid_rewrite bind_vis. reflexivity. cbn. rewrite bind_ret_l. destruct b; auto. Unshelve. apply tt. }
+       setoid_rewrite bind_trigger.
+       rewrite Hm2s2. setoid_rewrite bind_vis. apply eqit_Vis. intros [].
+       eapply eqit_bind'. reflexivity. intros [] [] _. apply eqit_Vis; intros [].
+Qed.
+
+Variant max_exception_label_coind_e l : forall A, (impExcE +' IOE) A -> Prop :=
+  | melce_print (e : IOE unit) : max_exception_label_coind_e l unit (inr1 e)
+  | melce_exc l' : leq l' l -> max_exception_label_coind_e l void (inl1 (Throw _ l'))
+.
+
+Definition max_exception_label_coind {R} l (t : itree _ R ) := itree_forall (max_exception_label_coind_e l) (fun _ => True) t.
+
+Lemma max_exception_label_coind_imp_ind_aux R l (t : itree _ R) : 
+  max_exception_label_coind l t -> forall l', raises_exception (Throw _ l') t -> leq l' l.
+Proof.
+  intros Hcoind l' Hraise. red in Hraise. destruct Hraise as [t' [Hconv Ht'] ].
+  generalize dependent t. induction Hconv; intros.
+  - rewrite H in Ht'. setoid_rewrite bind_ret_l in Ht'. setoid_rewrite bind_trigger in Ht'.
+    rewrite Ht' in Hcoind.  punfold Hcoind. clear Ht' H. red in Hcoind. inv Hcoind.
+    ITrace.inj_existT; subst. pclearbot. inv H1; auto.
+  - rewrite H in Ht'. setoid_rewrite bind_vis in Ht'. 
+    rewrite Ht' in Hcoind.
+    pinversion Hcoind; ITrace.inj_existT; subst.
+    eapply IHHconv; try apply H4. Unshelve. all: auto. reflexivity.
+Qed.
+
+Lemma max_exception_label_coind_imp_ind R lexn (m : stateT map (itree _ ) R)  :
+  (forall s, max_exception_label_coind lexn (m s)) -> max_exception_label lexn m. 
+Proof.
+  intros Hm. red. unfold can_raise_exception.
+  intros. destruct H as [s Hs]. revert Hs. apply max_exception_label_coind_imp_ind_aux; auto.
+Qed.
+
+Lemma max_exception_label_coind_flip_imp_ind R lexn (m : stateT map (itree _ ) R)  :
+   max_exception_label lexn m -> (forall s, max_exception_label_coind lexn (m s)). 
+Proof.
+  ginit. intros. red in H0. unfold can_raise_exception in H0.
+  assert (forall l', raises_exception (Throw _ l') (m s) -> leq l' lexn ).
+  { intros. apply H0. exists s. auto. }
+  clear H0. remember (m s) as t. clear Heqt. clear s m. generalize dependent t. gcofix CIH. intros.
+  destruct (observe t) eqn : Ht; symmetry in Ht; use_simpobs.
+  - rewrite Ht. gstep. constructor. auto.
+  - rewrite Ht. gstep. constructor. gfinal. left. eapply CIH; eauto.
+    assert (t ≈ t0). rewrite Ht. rewrite tau_eutt. reflexivity.
+    setoid_rewrite <- H. auto.
+  - rewrite Ht. setoid_rewrite Ht in H0.
+    destruct e.
+    + destruct i. gstep. constructor. 2 : intros []. constructor.
+      apply H0. exists (Ret tt). split. constructor; reflexivity.
+      setoid_rewrite bind_ret_l. setoid_rewrite bind_trigger.
+      apply eqit_Vis. intros [].
+    + destruct i. gstep. constructor. constructor.
+      intros. gfinal. left. eapply CIH; eauto.
+      intros. apply H0. red in H. destruct H as [t' [Hconv Ht'] ].
+      exists (Vis (inr1 (LabelledPrint s v) ) (fun _ => t') ). split.
+      * eapply conv_vis. reflexivity. auto. Unshelve. apply tt.
+      * setoid_rewrite bind_vis. apply eqit_Vis. destruct a. intros [].
+        apply Ht'.
+Qed.
+
