theories/Secure/SecurityImpExc/SecurityImpTypes.v
@@ -1,0 +1,654 @@
+From Coq Require Import
+     Arith.PeanoNat
+     Lists.List
+     Strings.String
+     Morphisms
+     Setoid
+     RelationClasses
+     Logic.Classical_Prop
+.
+
+From ExtLib Require Import
+     Data.String
+     Structures.Monad
+     Structures.Traversable
+     Data.List.
+
+From ITree Require Import
+     ITree
+     ITreeFacts
+     Events.MapDefault
+     Events.State
+     Events.StateFacts
+     Events.Exception
+     Events.ExceptionFacts
+     Core.Divergence
+     Dijkstra.TracesIT
+     Dijkstra.ITrace
+     Secure.SecureEqHalt
+     Secure.SecureEqEuttHalt
+     Secure.SecureEqWcompat
+     Secure.SecureEqBind
+     Secure.SecurityImpExc.SecurityImp
+     Secure.SecurityImpExc.SecurityImpHandler
+     Secure.StrongBisimProper
+     Secure.SecurityImpExc.RaiseException
+     Secure.SecurityImpExc.ITreeForall
+.
+
+
+Import Monads.
+Import MonadNotation.
+Local Open Scope monad_scope.
+Local Open Scope string_scope.
+
+Instance sense_preorder_in : Preorder := sense_preorder.
+
+Notation label := sensitivity.
+
+Definition labelled_equiv (Γ : privacy_map) (l : label) (σ1 σ2 : map)  : Prop :=
+  forall x, leq (Γ x) l -> σ1 x = σ2 x.
+
+Instance labelled_equit_equiv {Γ l} : Equivalence (labelled_equiv Γ l).
+Proof.
+  constructor; unfold labelled_equiv.
+  - red. intros; auto.
+  - red. intros. symmetry; auto.
+  - red. intros. rewrite H; auto.
+Qed.
+
+Definition label_eqit_secure_impstate  (b1 b2 : bool) (Γ : privacy_map) (l : label) {R1 R2 : Type} (RR : R1 -> R2 -> Prop )
+           (m1 : stateT map (itree (impExcE +' IOE)) R1) (m2 : stateT map (itree (impExcE +' IOE)) R2) : Prop :=
+  forall σ1 σ2, labelled_equiv Γ l σ1 σ2 -> eqit_secure sense_preorder priv_exc_io (product_rel (labelled_equiv Γ l) RR) b1 b2 l (m1 σ1) (m2 σ2).
+
+Definition label_state_sec_eutt {R1 R2} priv l (RR : R1 -> R2 -> Prop) m1 m2 :=
+  label_eqit_secure_impstate true true  priv l RR m1 m2.
+
+Definition sem_stmt (s : stmt) := interp_imp (denote_stmt s).
+
+Definition sem_expr (e : expr) := interp_imp (denote_expr e).
+
+Definition state_equiv {E R} (m1 m2 : stateT map (itree E) R) := forall (σ : map), m1 σ ≈ m2 σ.
+
+Instance proper_eutt_secure_eutt  {E R1 R2 RR Label priv l} : Proper (@eutt E R1 R1 eq ==> @eutt E R2 R2 eq ==> iff)
+                                                               (eqit_secure Label priv RR true true l).
+Proof.
+  eapply proper_eqit_secure_eqit.
+Qed.
+
+Instance proper_eq_itree_secure_eutt  {E R1 R2 RR Label priv l} : Proper (@eq_itree E R1 R1 eq ==> @eq_itree E R2 R2 eq ==> iff)
+                                                               (eqit_secure Label priv RR true true l).
+Proof.
+  repeat intro. assert (x ≈ y). rewrite H. reflexivity. 
+  assert (x0 ≈ y0). rewrite H0. reflexivity. rewrite H1. rewrite H2. tauto.
+Qed.
+
+Instance proper_state_equiv_label_state_sec_eutt {R1 R2 RR priv l} : Proper (@state_equiv _ R1 ==> @state_equiv _ R2 ==> iff) (@label_state_sec_eutt R1 R2 priv l RR).
+Proof.
+  repeat intro. split.
+  - intros. do 2 red in H1. do 2 red. intros. red in H0. specialize (H0 σ2). red in H.
+    specialize (H σ1). eapply proper_eutt_secure_eutt; eauto. symmetry. auto. symmetry. auto.
+  - intros. intros. do 2 red in H1. do 2 red. intros. red in H0. specialize (H0 σ2). red in H.
+    specialize (H σ1).  eapply proper_eutt_secure_eutt; eauto.
+Qed.
+(* this is the notion of finiteness I want to work with 
+   note that the linearness of these ITrees is part of what makes it enough
+   otherwise I would need a more Forall like coinductive predicate
+   I want to move a bunch of this raise exception stuff to another file
+*)
+
+Definition state_try_catch {E R} (m : stateT map (itree (impExcE +' E) ) R)  := 
+                                   fun σ => try_catch (m σ).
+
+
+
+
+Context (Γ : privacy_map).
+
+Variant secure_stmt_at_label (observer pc lexn : label) (s : stmt) : Prop :=
+  | ssal_leq : (leq pc observer) -> label_state_sec_eutt Γ observer eq (sem_stmt s) (sem_stmt s) -> secure_stmt_at_label observer pc lexn s
+  | ssal_nleq : (~ leq pc observer) -> label_state_sec_eutt Γ observer top2 (sem_stmt s) (ret tt) -> secure_stmt_at_label observer pc lexn s.
+
+
+Variant secure_expr_at_label (observer protection: label ) (e : expr) : Prop :=
+  | seal_leq : (leq protection observer) -> label_state_sec_eutt Γ observer eq (sem_expr e) (sem_expr e) -> 
+               secure_expr_at_label observer protection e
+  | seal_nleq : (~leq protection observer) -> (exists n:value, label_state_sec_eutt Γ observer top2 (sem_expr e) (ret n)) ->
+                secure_expr_at_label observer protection e
+.
+
+Definition secure_expr l e := forall observer, secure_expr_at_label observer l e.
+
+Definition secure_stmt pc lexn c := forall observer, secure_stmt_at_label observer pc lexn c.
+
+Inductive well_typed_expr : sensitivity -> expr -> Prop :=
+  | wte_lit l n : well_typed_expr l (Lit n)
+  | wte_var x l : leq (Γ x) l -> well_typed_expr l (Var x)
+  | wte_plus l1 l2 e1 e2 : well_typed_expr l1 e1 -> well_typed_expr l2 e2 ->
+                           well_typed_expr (join l1 l2) (Plus e1 e2)
+  | wte_min l1 l2 e1 e2 : well_typed_expr l1 e1 -> well_typed_expr l2 e2 ->
+                           well_typed_expr (join l1 l2) (Minus e1 e2)
+  | wte_mult l1 l2 e1 e2 : well_typed_expr l1 e1 -> well_typed_expr l2 e2 ->
+                           well_typed_expr (join l1 l2) (Mult e1 e2)
+.
+
+
+Inductive well_typed_stmt : sensitivity -> sensitivity -> stmt -> Prop :=
+  | wts_manual pc lexn s : secure_stmt pc lexn s -> well_typed_stmt pc lexn s
+  | wts_skip pc : well_typed_stmt pc Public Skip
+  | wts_seq pc lexn1 lexn2 s1 s2 : well_typed_stmt pc lexn1 s1 -> well_typed_stmt (join lexn1 pc) lexn2 s2 ->
+                                   well_typed_stmt pc (join lexn1 lexn2) (Seq s1 s2)
+  | wts_assign pc l x e : well_typed_expr l e -> leq (join l pc) (Γ x) ->
+                          well_typed_stmt pc Public (Assign x e)
+  | wts_print pc le lp e : well_typed_expr le e -> leq (join le pc) lp ->
+                           well_typed_stmt pc Public (Output lp e)
+  | wts_if pc le lexn1 lexn2 e s1 s2 : well_typed_expr le e -> well_typed_stmt (join pc le) lexn1 s1 -> well_typed_stmt (join pc le) lexn2 s2 ->
+                                       well_typed_stmt pc (join lexn1 lexn2) (If e s1 s2)
+  | wts_while lexn e s : well_typed_expr Public e -> well_typed_stmt Public lexn s ->
+                         well_typed_stmt Public lexn (While e s)
+  | wts_raise pc l : leq pc l -> well_typed_stmt pc l (Raise l)
+  | wts_try pc lexn1 lexn2 s1 s2 : well_typed_stmt pc lexn1 s1 -> well_typed_stmt (join lexn1 pc) lexn2 s2 ->
+                                   well_typed_stmt pc lexn2 (TryCatch s1 s2)
+.
+
+
+
+Lemma well_typed_expr_upward_close l1 l2 e : leq l1 l2 -> well_typed_expr l1 e -> well_typed_expr l2 e.
+Proof.
+  revert l1 l2.
+  induction e; intros; try inv H0.
+  - constructor. eapply leq_sense_trans; eauto.
+  - constructor.
+  - assert (l2 = join l2 l2). destruct l2; auto. rewrite H0. constructor.
+    + eapply IHe1; eauto. eapply IHe1; eauto. apply leq_sense_join_l.
+    + eapply IHe2; eauto. eapply IHe2; eauto. apply leq_sense_join_r.
+  - assert (l2 = join l2 l2). destruct l2; auto. rewrite H0. constructor.
+    + eapply IHe1; eauto. eapply IHe1; eauto. apply leq_sense_join_l.
+    + eapply IHe2; eauto. eapply IHe2; eauto. apply leq_sense_join_r.
+  - assert (l2 = join l2 l2). destruct l2; auto. rewrite H0. constructor.
+    + eapply IHe1; eauto. eapply IHe1; eauto. apply leq_sense_join_l.
+    + eapply IHe2; eauto. eapply IHe2; eauto. apply leq_sense_join_r.
+Qed.
+
+Lemma expr_only_ret_aux1 e observer: forall (n : nat), label_state_sec_eutt Γ observer top2 (sem_expr e) (ret n) .
+Proof.
+  do 2 red. induction e; intros; unfold sem_expr; cbn; unfold interp_imp.
+  - eapply proper_eutt_secure_eutt; try apply interp_state_trigger; try reflexivity. cbn.
+    apply secure_eqit_ret. split; cbv; auto.
+  - rewrite interp_state_ret. apply secure_eqit_ret. split; cbv; auto.
+  - repeat setoid_rewrite interp_state_bind.
+    match goal with |- eqit_secure _ _ _ _ _ _ _ ?t =>
+    assert ( t ≈ ITree.bind (Ret (σ2, n)) (fun st : map * nat => ITree.bind (Ret (fst st, n) ) (fun st : map * nat => Ret (fst st,n))  )  ) end.
+    { repeat rewrite bind_ret_l. reflexivity. }
+    eapply proper_eutt_secure_eutt; try apply H0; try reflexivity.
+    eapply secure_eqit_bind; try apply IHe1; eauto. intros [? ?] [? ?] [? ?]. cbn in *.
+    eapply secure_eqit_bind; try apply IHe2; eauto. intros [? ?] [? ?] [? ?]. cbn in *.
+    setoid_rewrite interp_state_ret. apply secure_eqit_ret; split; auto.
+  - repeat setoid_rewrite interp_state_bind.
+    match goal with |- eqit_secure _ _ _ _ _ _ _ ?t =>
+    assert ( t ≈ ITree.bind (Ret (σ2, n)) (fun st : map * nat => ITree.bind (Ret (fst st, n) ) (fun st : map * nat => Ret (fst st,n))  )  ) end.
+    { repeat rewrite bind_ret_l. reflexivity. }
+    eapply proper_eutt_secure_eutt; try apply H0; try reflexivity.
+    eapply secure_eqit_bind; try apply IHe1; eauto. intros [? ?] [? ?] [? ?]. cbn in *.
+    eapply secure_eqit_bind; try apply IHe2; eauto. intros [? ?] [? ?] [? ?]. cbn in *.
+    setoid_rewrite interp_state_ret. apply secure_eqit_ret; split; auto.
+  - repeat setoid_rewrite interp_state_bind.
+    match goal with |- eqit_secure _ _ _ _ _ _ _ ?t =>
+    assert ( t ≈ ITree.bind (Ret (σ2, n)) (fun st : map * nat => ITree.bind (Ret (fst st, n) ) (fun st : map * nat => Ret (fst st,n))  )  ) end.
+    { repeat rewrite bind_ret_l. reflexivity. }
+    eapply proper_eutt_secure_eutt; try apply H0; try reflexivity.
+    eapply secure_eqit_bind; try apply IHe1; eauto. intros [? ?] [? ?] [? ?]. cbn in *.
+    eapply secure_eqit_bind; try apply IHe2; eauto. intros [? ?] [? ?] [? ?]. cbn in *.
+    setoid_rewrite interp_state_ret. apply secure_eqit_ret; split; auto.
+Qed.
+
+Lemma expr_only_ret e observer:  exists n : value, label_state_sec_eutt Γ observer top2 (sem_expr e) (ret n) .
+Proof.
+  exists 0. apply expr_only_ret_aux1.
+Qed.
+
+
+Lemma well_typed_expr_correct l e : well_typed_expr l e -> secure_expr l e.
+Proof.
+  revert l. red. induction e; intros l Htype observer.
+  - inv Htype. case_leq l observer.
+    + left; auto. unfold sem_expr. cbn. unfold interp_imp.
+      do 2 red. intros. eapply proper_eutt_secure_eutt; try apply interp_state_trigger.
+      cbn.
+      unfold get. apply secure_eqit_ret; split; auto. cbn.
+      red in H0. apply H0. eapply leq_sense_trans; eauto.
+    + right; auto. apply expr_only_ret.
+  - case_leq l observer.
+    + left; auto. unfold sem_expr. cbn. unfold interp_imp. do 2 red.
+      intros. setoid_rewrite interp_state_ret. apply secure_eqit_ret.
+      split; auto.
+    + right; auto. exists 0. unfold sem_expr. cbn. unfold interp_imp. do 2 red.
+      intros. setoid_rewrite interp_state_ret. apply secure_eqit_ret. split; auto.
+      cbv. auto.
+  - inv Htype.
+    assert (well_typed_expr (join l1 l2) e1 ). eapply well_typed_expr_upward_close; eauto. apply leq_sense_join_l.
+    assert (well_typed_expr (join l1 l2) e2 ). eapply well_typed_expr_upward_close; eauto. apply leq_sense_join_r.
+    apply IHe1 with (observer := observer) in H.
+    apply IHe2 with (observer := observer) in H0. inv H; inv H0; try contradiction.
+    + left; auto.
+      unfold sem_expr. cbn. unfold interp_imp. do 2 red. intros.
+      repeat setoid_rewrite interp_state_bind.
+      eapply secure_eqit_bind. 2 : eapply H4; eauto.
+      intros [s3 r1] [s4 r2] Hprod. destruct Hprod. cbn in *. subst.
+      eapply secure_eqit_bind. 2 : eapply H5; eauto.
+      intros [? ?] [? ?] [? ?]. cbn in *. subst. setoid_rewrite interp_state_ret.
+      apply secure_eqit_ret. split; auto.
+    + right; auto. apply expr_only_ret.
+  - inv Htype.
+    assert (well_typed_expr (join l1 l2) e1 ). eapply well_typed_expr_upward_close; eauto. apply leq_sense_join_l.
+    assert (well_typed_expr (join l1 l2) e2 ). eapply well_typed_expr_upward_close; eauto. apply leq_sense_join_r.
+    apply IHe1 with (observer := observer) in H.
+    apply IHe2 with (observer := observer) in H0. inv H; inv H0; try contradiction.
+    + left; auto.
+      unfold sem_expr. cbn. unfold interp_imp. do 2 red. intros.
+      repeat setoid_rewrite interp_state_bind.
+      eapply secure_eqit_bind. 2 : eapply H4; eauto.
+      intros [s3 r1] [s4 r2] Hprod. destruct Hprod. cbn in *. subst.
+      eapply secure_eqit_bind. 2 : eapply H5; eauto.
+      intros [? ?] [? ?] [? ?]. cbn in *. subst. setoid_rewrite interp_state_ret.
+      apply secure_eqit_ret. split; auto.
+    + right; auto. apply expr_only_ret.
+  - inv Htype.
+    assert (well_typed_expr (join l1 l2) e1 ). eapply well_typed_expr_upward_close; eauto. apply leq_sense_join_l.
+    assert (well_typed_expr (join l1 l2) e2 ). eapply well_typed_expr_upward_close; eauto. apply leq_sense_join_r.
+    apply IHe1 with (observer := observer) in H.
+    apply IHe2 with (observer := observer) in H0. inv H; inv H0; try contradiction.
+    + left; auto.
+      unfold sem_expr. cbn. unfold interp_imp. do 2 red. intros.
+      repeat setoid_rewrite interp_state_bind.
+      eapply secure_eqit_bind. 2 : eapply H4; eauto.
+      intros [s3 r1] [s4 r2] Hprod. destruct Hprod. cbn in *. subst.
+      eapply secure_eqit_bind. 2 : eapply H5; eauto.
+      intros [? ?] [? ?] [? ?]. cbn in *. subst. setoid_rewrite interp_state_ret.
+      apply secure_eqit_ret. split; auto.
+    + right; auto. apply expr_only_ret.
+Qed.
+
+Lemma state_secure_eutt_ret_aux:
+  forall R t1 t2 (observer : sensitivity) (r1 r2 : R),
+    (forall σ1 σ2 : map,
+        labelled_equiv Γ observer σ1 σ2 ->
+        eqit_secure sense_preorder priv_exc_io (product_rel (labelled_equiv Γ observer) (@top2 R R)) true
+                    true observer (interp_imp t1 σ1) (Ret(σ2,r1))) ->
+    (forall σ1 σ2 : map,
+        labelled_equiv Γ observer σ1 σ2 ->
+        eqit_secure sense_preorder priv_exc_io (product_rel (labelled_equiv Γ observer) (@top2 R R)) true
+                    true observer (interp_imp t2 σ1) (Ret(σ2,r2))) ->
+    forall σ1 σ2 : map,
+      labelled_equiv Γ observer σ1 σ2 ->
+      eqit_secure sense_preorder priv_exc_io (product_rel (labelled_equiv Γ observer) top2) true
+                  true observer (interp_state handle_imp t1 σ1)
+                  (interp_state handle_imp t2 σ2).
+Proof.
+  intros R t1 t2 observer r1 r2 Hr1 Hr2 s1 s2 Hs12.
+  set ((product_rel (labelled_equiv Γ observer) top2)) as Rst.
+  apply eqit_secure_RR_imp with (RR1 := rcompose Rst Rst).
+  { intros [? ?] [? ?] [? ?]. destruct r3. cbn in *. unfold Rst in *.
+    split. 2 : cbv; auto. destruct REL1 as [REL1 _]. destruct REL2 as [REL2 _].
+    cbn in *. etransitivity; eauto. }
+  eapply eqit_secure_trans; eauto. eapply eqit_secure_sym.
+  apply eqit_secure_RR_imp with (RR1 := Rst).
+  { intros. split. 2 : cbv; auto. unfold Rst in PR. destruct PR.
+    symmetry. auto. }
+  assert (eqit_secure sense_preorder priv_exc_io Rst true true observer (Ret (s2, r2) ) (Ret (s2,r1))).
+  { apply secure_eqit_ret. unfold Rst in *. split; auto; cbv; auto. }
+  apply eqit_secure_RR_imp with (RR1 := rcompose Rst Rst).
+  { intros [? ?] [? ?] [? ?]. destruct r3. cbn in *. unfold Rst in *.
+    split. 2 : cbv; auto. destruct REL1 as [REL1 _]. destruct REL2 as [REL2 _].
+    cbn in *. etransitivity; eauto. }
+  eapply eqit_secure_trans; try apply Hr2; eauto. reflexivity. 
+Qed.
+
+Lemma update_labelled_equiv_invisible:
+  forall (x : var) (observer : sensitivity),
+    ~ leq (Γ x) observer ->
+    forall (σ1 : map) (v : value) (σ2 : map),
+      labelled_equiv Γ observer σ1 σ2 -> labelled_equiv Γ observer (update x v σ1) (σ2).
+Proof.
+  intros x observer H σ1 v σ2 H2.
+  red. red in H2. intros.
+  unfold update. destruct (x =? x0) eqn : Heq; auto.
+  exfalso. apply H. apply eqb_eq in Heq. subst; auto.
+Qed.
+
+Lemma update_labelled_equiv_visible:
+  forall (x : var) (observer : sensitivity),
+    leq (Γ x) observer ->
+    forall (σ1 : map) (v : value) (σ2 : map),
+      labelled_equiv Γ observer σ1 σ2 -> labelled_equiv Γ observer (update x v σ1) (update x v σ2).
+Proof.
+  intros x observer H σ1 v σ2 H2.
+  red. red in H2. intros. unfold update. 
+  destruct (x =? x0) eqn : Heq; auto.
+Qed.
+
+Lemma assign_well_typed_correct x e pc lexn : well_typed_stmt pc lexn (Assign x e) -> secure_stmt pc lexn (Assign x e).
+Proof.
+  red. intros. 
+  inv H; auto.
+  assert (Hpc : leq pc (Γ x) ).
+  { eapply leq_sense_trans; eauto. apply leq_sense_join_r. }
+  assert (Hl : leq l (Γ x) ).
+  { eapply leq_sense_trans; try apply H5. apply leq_sense_join_l. }
+  assert (He : well_typed_expr (Γ x) e ).
+  { eapply well_typed_expr_upward_close with (l2:= Γ x); eauto. }
+  apply well_typed_expr_correct in He. 
+  specialize ( He observer). inv He.
+  - left. eapply leq_sense_trans; eauto.
+    do 2 red in H0. do 2 red. intros. unfold sem_stmt.
+    cbn. unfold interp_imp. setoid_rewrite interp_state_bind.
+    eapply secure_eqit_bind; eauto. intros [? ?] [? ?] [? ?].
+    cbn in H2, H3. subst. eapply proper_eutt_secure_eutt; try apply interp_state_trigger.
+    cbn. apply secure_eqit_ret; split; auto. cbn. apply update_labelled_equiv_visible; auto. 
+  - case_leq pc observer.
+    + left; auto.
+      destruct H0 as [n Hn]. unfold sem_stmt.
+      cbn. unfold interp_imp. do 2 red. intros. setoid_rewrite interp_state_bind.
+      do 2 red in Hn.
+      eapply secure_eqit_bind with (RR := product_rel (labelled_equiv Γ observer) top2 ); eauto.
+      2 : { eapply state_secure_eutt_ret_aux; try apply Hn; auto. }
+      intros [? ?] [? ?] [? ?]. clear H3. cbn in H2. cbn.
+      eapply proper_eutt_secure_eutt; try apply interp_state_trigger.
+      cbn. apply secure_eqit_ret. split. 2 : cbv; auto. cbn.
+      apply update_labelled_equiv_invisible; auto. symmetry.
+      apply update_labelled_equiv_invisible;  auto.
+      symmetry; auto.
+    + right; auto.
+      destruct H0 as [n Hn]. unfold sem_stmt. cbn.
+      do 2 red in Hn. do 2 red. intros. unfold sem_stmt. cbn.
+      setoid_rewrite interp_state_bind.
+      match goal with |- eqit_secure _ _ _ _ _ _ _ ?t =>
+                      assert (t ≈ (ITree.bind (Ret (σ2, n)) (fun st => Ret (fst st, tt) ))) end.
+      rewrite bind_ret_l. reflexivity.
+      eapply proper_eutt_secure_eutt; try apply H2; try reflexivity.
+      eapply secure_eqit_bind; try apply Hn; eauto.
+      intros [? ?] [? ?] [? ?]. cbn in H3.
+      eapply proper_eutt_secure_eutt; try apply interp_state_trigger; try reflexivity.
+      cbn.
+      apply secure_eqit_ret; split; auto. 
+      cbn. apply update_labelled_equiv_invisible; auto.
+Qed.
+
+Lemma expr_only_ret' e s : exists n, sem_expr e s ≈ Ret(s, n).
+Proof.
+  unfold sem_expr, interp_imp. cbn.
+  induction e.
+  - cbn. setoid_rewrite interp_state_trigger. cbn. repeat setoid_rewrite bind_ret_l.
+    cbn. eexists; reflexivity.
+  - cbn. setoid_rewrite interp_state_ret. 
+    eexists; reflexivity.
+  - destruct IHe1 as [n1 IHn1]. destruct IHe2 as [n2 IHn2].
+    cbn. setoid_rewrite interp_state_bind. setoid_rewrite IHn1.
+    setoid_rewrite bind_ret_l. setoid_rewrite interp_state_bind. setoid_rewrite IHn2.
+    setoid_rewrite bind_ret_l. setoid_rewrite interp_state_ret.
+    eexists; reflexivity.
+  - destruct IHe1 as [n1 IHn1]. destruct IHe2 as [n2 IHn2].
+    cbn. setoid_rewrite interp_state_bind. setoid_rewrite IHn1.
+    setoid_rewrite bind_ret_l. setoid_rewrite interp_state_bind. setoid_rewrite IHn2.
+    setoid_rewrite bind_ret_l. setoid_rewrite interp_state_ret.
+    eexists; reflexivity.
+  - destruct IHe1 as [n1 IHn1]. destruct IHe2 as [n2 IHn2].
+    cbn. setoid_rewrite interp_state_bind. setoid_rewrite IHn1.
+    setoid_rewrite bind_ret_l. setoid_rewrite interp_state_bind. setoid_rewrite IHn2.
+    setoid_rewrite bind_ret_l. setoid_rewrite interp_state_ret.
+    eexists; reflexivity.
+Qed.
+
+Lemma assign_only_ret e x σ : exists σ', sem_stmt (Assign x e) σ ≈ Ret (σ', tt).
+Proof.
+  unfold sem_stmt, interp_imp. cbn.
+  setoid_rewrite interp_state_bind. specialize (expr_only_ret' e σ) as He.
+  destruct He as [n Hn]. setoid_rewrite Hn. setoid_rewrite bind_ret_l.
+  setoid_rewrite interp_state_trigger. cbn. eexists; reflexivity.
+Qed.
+
+
+
+Lemma assign_max_exception_label x e lexn : max_exception_label lexn (sem_stmt (Assign x e) ).
+Proof.
+  red. intros. red in H. destruct H as [σ Hσ]. 
+  specialize (assign_only_ret e x σ) as Haor. destruct Haor as [σ' Haor].
+  setoid_rewrite Haor in Hσ. exfalso. eapply raises_exception_ret; eauto.
+Qed.
+
+
+From Paco Require Import paco.
+Lemma output_max_exception_label e lexn l : max_exception_label lexn (sem_stmt (Output l e ) ).
+Proof.
+  red. intros. exfalso. red in H. destruct H as [s Hs].
+  unfold sem_stmt, interp_imp in Hs. cbn in Hs. setoid_rewrite interp_state_bind in Hs.
+  specialize (expr_only_ret' e s) as Hes. destruct Hes as [n Hn]. rewrite Hn in Hs.
+  rewrite bind_ret_l in Hs. setoid_rewrite interp_state_trigger in Hs. cbn in Hs.
+  rewrite bind_trigger in Hs. red in Hs. destruct Hs as [t' [Hconv Ht'] ].
+  symmetry in Ht'. apply eqit_inv_bind_vis in Ht'.
+  destruct Ht' as [Ht' | Ht'].
+  - destruct Ht' as [kxa [Heq Hbind] ]. 
+    rewrite Heq in Hconv. inversion Hconv.
+    + symmetry in H. eapply eqit_inv_ret_vis; eauto.
+    + pinversion H; subst; ITrace.inj_existT; subst.
+      rewrite <- REL in H0. clear H REL. destruct b. specialize (Hbind tt).
+      inversion H0.
+      * rewrite H in Hbind. rewrite bind_ret_l in Hbind. setoid_rewrite bind_trigger in Hbind.
+        pinversion Hbind.
+      * setoid_rewrite H in Hbind. setoid_rewrite bind_vis in Hbind. pinversion Hbind.
+  - destruct Ht' as [ [] [? ?] ]. setoid_rewrite bind_trigger in H0.
+    pinversion H0; subst;  ITrace.inj_existT; subst. discriminate.
+Qed.
+
+
+Lemma output_well_typed_correct l1 lexn pc e : 
+  well_typed_stmt pc lexn (Output l1 e) -> secure_stmt pc lexn (Output l1 e).
+Proof.
+  red. intros. inv H; auto.
+  assert (Hle : leq le l1).
+  { eapply leq_sense_trans; eauto. apply leq_sense_join_l. }
+  assert (Hpc : leq pc l1).
+  { eapply leq_sense_trans; try apply H5. apply leq_sense_join_r. }
+  assert (He : well_typed_expr l1 e ).
+  { eapply well_typed_expr_upward_close with (l1 := le); eauto. }
+  apply well_typed_expr_correct in He. specialize (He observer).
+  inv He.
+  - assert (Hobs : leq pc observer). eapply leq_sense_trans; eauto.
+    left; auto.
+    do 2 red in H0. do 2 red. intros. unfold sem_stmt. cbn.
+    unfold interp_imp. setoid_rewrite interp_state_bind.
+    eapply secure_eqit_bind; eauto. intros [? ?] [? ?] [? ?].
+    cbn in H2, H3. subst. cbn. eapply proper_eutt_secure_eutt; try apply interp_state_trigger.
+    cbn. setoid_rewrite bind_trigger. cbn.
+    apply eqit_secure_public_Vis; try apply H.
+    intros []. apply secure_eqit_ret; auto.
+  - case_leq pc observer.
+    + left; auto. destruct H0 as [n Hn]. do 2 red in Hn. cbn in Hn.
+      unfold sem_stmt. cbn. unfold interp_imp. do 2 red. 
+      intros. setoid_rewrite interp_state_bind.
+      eapply secure_eqit_bind with (RR := product_rel (labelled_equiv Γ observer) top2 ); eauto.
+      2 : { eapply state_secure_eutt_ret_aux; try apply Hn; auto. }
+      intros [? ?] [? ?] [? ?]. cbn in H2. clear H3. cbn.
+      eapply proper_eutt_secure_eutt; try apply interp_state_trigger.
+      cbn. setoid_rewrite bind_trigger. apply eqit_secure_private_VisLR; auto.
+      constructor; apply tt. constructor; apply tt. intros [] [].
+      apply secure_eqit_ret. split; auto.
+    + right; auto. destruct H0 as [n Hn]. do 2 red in Hn.
+      do 2 red. intros. unfold sem_stmt. cbn.
+      unfold interp_imp. setoid_rewrite interp_state_bind.
+      match goal with |- eqit_secure _ _ _ _ _ _ _ ?t =>
+                      assert (t ≈ (ITree.bind (Ret (σ2, n)) (fun st => Ret (fst st, tt) ))) end.
+      rewrite bind_ret_l. reflexivity.
+      eapply proper_eutt_secure_eutt; try apply H2; try reflexivity.
+      eapply secure_eqit_bind; try apply Hn; eauto.
+      intros [? ?] [? ?] [? ?]. cbn. 
+      eapply proper_eutt_secure_eutt; try apply interp_state_trigger; try reflexivity.
+      cbn. setoid_rewrite bind_trigger. cbn.
+      apply eqit_secure_private_VisL; auto. constructor; apply tt.
+      intros []. apply secure_eqit_ret; auto.
+Qed.
+
+Lemma seq_well_typed_correct pc lexn1 lexn2 s1 s2 : 
+  secure_stmt pc lexn1 s1 -> secure_stmt (join lexn1 pc) lexn2 s2 ->
+  secure_stmt pc (join lexn1 lexn2) (Seq s1 s2).
+Proof.
+  intros Hc1 Hc2. red. intros.
+  specialize (Hc1 observer) as Hc1obs. specialize (Hc2 observer) as Hc2obs.
+  inv Hc1obs.
+  - do 2 red in H0. left; auto. unfold sem_stmt.
+    cbn. unfold interp_imp. do 2 red. intros. setoid_rewrite interp_state_bind.
+    eapply secure_eqit_bind; eauto. intros [? [] ] [? [] ] [? ?].
+    clear H3. cbn in H2. cbn.
+    inv Hc2obs; try apply H4; auto.
+    do 2 red in H4. 
+    eapply eqit_secure_RR_imp with (RR1 := product_rel (labelled_equiv Γ observer) top2 ).
+    { intros [ ? [] ] [? [] ] [? ?] . split; auto. }
+    eapply state_secure_eutt_ret_aux; try apply H4; eauto.
+    (* I think this ends up being fine*)
+  - right; auto. unfold sem_stmt, interp_imp. cbn. do 2 red. intros.
+    setoid_rewrite interp_state_bind.
+    inv Hc2obs.
+    { exfalso. apply H. eapply leq_sense_trans; try apply H2. apply leq_sense_join_r. }
+    match goal with |- eqit_secure _ _ _ _ _ _ _ ?t =>
+                      assert (t ≈ (ITree.bind (Ret (σ2, tt)) (fun st => Ret (fst st, tt) ))) end.
+    rewrite bind_ret_l. reflexivity.
+    eapply proper_eutt_secure_eutt; try apply H4; try reflexivity.
+    eapply secure_eqit_bind; try eapply H0; auto.
+    intros [? ?] [? ?] [? ?]. apply H3; auto.
+Qed.
+
+
+Lemma if_well_typed_correct pc le lexn1 lexn2 e s1 s2 :
+  secure_expr le e -> secure_stmt (join pc le) lexn1 s1 -> secure_stmt (join pc le) (lexn2) s2 ->
+  secure_stmt pc (join lexn1 lexn2) (If e s1 s2).
+Proof.
+  intros He Hc1 Hc2. red. intros.
+  specialize (Hc1 observer) as Hc1obs. specialize (Hc2 observer) as Hc2obs.
+  specialize (He observer).
+  inv Hc1obs; inv Hc2obs; try contradiction.
+  - left. eapply leq_sense_trans; eauto. apply leq_sense_join_l.
+    inv He. 2 : { exfalso. apply H3. eapply leq_sense_trans; eauto. apply leq_sense_join_r. }
+    unfold sem_stmt, interp_imp.
+    cbn. do 2 red. intros. setoid_rewrite interp_state_bind. eapply secure_eqit_bind; try apply H4; auto.
+    intros [? ?] [? ?] [? ?]. cbn in H6, H7. subst. cbn. destruct v0; eauto.
+  - case_leq pc observer.
+    + left; auto. unfold sem_stmt, interp_imp. cbn. do 2 red. intros.
+      setoid_rewrite interp_state_bind.
+      inv He; try contradiction.
+      * eapply secure_eqit_bind; try apply H5; eauto.
+        intros [? ?] [? ?] [? ?]. cbn in H8, H7. cbn. subst. do 2 red in H0, H2.
+        eapply eqit_secure_RR_imp with (RR1 := product_rel (labelled_equiv Γ observer) top2 ).
+        { intros [? [] ] [? [] ] [? ?]. split; auto. } 
+        destruct v0; try eapply  state_secure_eutt_ret_aux; cbn in *; eauto.
+      * destruct H6 as [n Hn]. do 2 red in Hn. 
+        eapply secure_eqit_bind; try eapply  state_secure_eutt_ret_aux; cbn in Hn; eauto.
+        intros [? ?] [? ?] [? ?]. cbn. cbn in H6.
+        eapply eqit_secure_RR_imp with (RR1 := product_rel (labelled_equiv Γ observer) top2 ).
+        { intros [? [] ] [? [] ] [? ?]. split; auto. } 
+        destruct v; destruct v0;
+        try eapply state_secure_eutt_ret_aux; try apply H0; try apply H2; eauto.
+     + right; auto. do 2 red. intros. unfold sem_stmt, interp_imp. cbn.
+       setoid_rewrite interp_state_bind.
+       match goal with |- eqit_secure _ _ _ _ _ _ _ ?t =>
+                      assert (t ≈ (ITree.bind (Ret (σ2, 0)) (fun st => Ret (fst st, tt) ))) end.
+       rewrite bind_ret_l. reflexivity.
+       eapply proper_eutt_secure_eutt; try apply H5; try reflexivity.
+       inv He.
+       * eapply secure_eqit_bind with (RR := product_rel (labelled_equiv Γ observer) top2) .
+         2 : { apply expr_only_ret_aux1; auto. }
+         intros [? ?] [? ?] [? ?]. cbn. destruct v; cbn in *; eauto.
+       * destruct H7. eapply secure_eqit_bind; try apply expr_only_ret_aux1; auto.
+         intros [? ?] [? ?] [? ?]. cbn. destruct v; cbn in *; eauto.
+Qed.
+
+Lemma if_max_label lexn1 lexn2 e s1 s2: max_exception_label lexn1 (sem_stmt s1) -> max_exception_label lexn2 (sem_stmt s2) ->
+                                        max_exception_label (join lexn1 lexn2) (sem_stmt (If e s1 s2)).
+Proof.
+  intros Hc1 Hc2. unfold sem_stmt, interp_imp. cbn. red. intros. red in H.
+  destruct H as [s Hs]. red in Hs. destruct Hs as [t' [Hconv Ht'] ].
+  setoid_rewrite interp_state_bind in Ht'. specialize (expr_only_ret' e s) as [n Hn].
+  rewrite Hn in Ht'. rewrite bind_ret_l in Ht'. cbn in Ht'. destruct n.
+  + enough (leq l' lexn2). eapply leq_sense_trans; eauto. apply leq_sense_join_r.
+    apply Hc2. exists s. red. exists t'. split; auto.
+  + enough (leq l' lexn1). eapply leq_sense_trans; eauto. apply leq_sense_join_l.
+    apply Hc1. exists s. red. exists t'. split; auto.
+Qed.
+
+(* maybe it would be easier to solve this problem in a more abstract way with monads rather than stmts*)
+Lemma while_max_label lexn e s : max_exception_label lexn (sem_stmt s) ->
+                                 max_exception_label lexn (sem_stmt (While e s)).
+Proof.
+  intros Hc. apply max_exception_label_coind_imp_ind. intros.
+  assert (forall σ, max_exception_label_coind lexn (sem_stmt s σ)  ).
+  apply max_exception_label_coind_flip_imp_ind; auto. 
+  unfold sem_stmt, interp_imp. cbn. unfold while.
+  specialize @interp_state_iter' as Hisi. red in Hisi. 
+  setoid_rewrite Hisi.
+  unfold Basics.iter, MonadIter_stateT0, Basics.iter, MonadIter_itree.
+  cbn. eapply itree_forall_iter_ev. intros [s' [] ].
+  setoid_rewrite interp_state_bind. cbn. specialize (expr_only_ret' e s') as [n Hn].
+  rewrite Hn. rewrite bind_ret_l. cbn. destruct n.
+  - rewrite interp_state_ret. rewrite bind_ret_l. cbn. pfold. constructor. auto.
+  - apply itree_forall_bind with (PS := fun _ => True).
+    + setoid_rewrite interp_state_bind. 
+      apply itree_forall_bind with (PS := fun _ => True); try apply H.
+      intros . setoid_rewrite interp_state_ret. pfold. constructor. auto.
+    + intros. pfold. constructor. auto.
+Qed.
+
+Lemma while_well_typed_correct lexn e s :
+  secure_expr Public e -> secure_stmt Public lexn s ->
+  secure_stmt Public lexn (While e s).
+Proof.
+  intros He Hc. red. intros.
+  assert (leq Public observer).
+  { destruct observer; cbv; auto. }
+  specialize (He observer).
+  specialize (Hc observer).
+  inv He; inv Hc; try contradiction.
+  left; auto. unfold sem_stmt, interp_imp. cbn. unfold while.
+  specialize @interp_state_iter' as Hisi. red in Hisi. do 2 red. intros.
+  setoid_rewrite Hisi. eapply secure_eqit_iter with (RA := product_rel (labelled_equiv Γ observer) eq).
+  { split; auto. }
+  intros [? [] ] [? [] ] [? ?]. cbn.
+  setoid_rewrite interp_state_bind. setoid_rewrite bind_bind.
+  eapply secure_eqit_bind; try apply H1; auto.
+  intros [? ?] [? ?] [? ?]. cbn. cbn in H7, H8; subst. destruct v0.
+  - setoid_rewrite interp_state_ret. setoid_rewrite bind_ret_l. cbn.
+    apply secure_eqit_ret. constructor. split; auto.
+  - setoid_rewrite interp_state_bind. setoid_rewrite bind_bind.
+    eapply secure_eqit_bind; try apply H3; auto.
+    intros [? [] ] [? [] ] [? ?]. cbn. cbn in H8.
+    setoid_rewrite interp_state_ret. setoid_rewrite bind_ret_l. cbn.
+    apply secure_eqit_ret. constructor. split; auto.
+Qed.
+
+
+Lemma try_catch_well_typed_correct lexn1 lexn2 s1 s2 pc :
+  secure_stmt pc lexn1 s1 -> max_exception_label lexn1 (sem_stmt s1) ->
+  secure_stmt (join pc lexn1) lexn2 s2 -> max_exception_label lexn2 (sem_stmt s2) ->
+  secure_stmt pc lexn2 (TryCatch s1 s2).
+Proof.
+  intros Hc1 Hec1 Hc2 Hec2. red. intros. specialize (Hc1 observer).
+  inv Hc1.
+  - left; auto. unfold sem_stmt. cbn. unfold interp_imp.
+    do 2 red. intros. do 2 red in H0. apply H0 in H1.
+    case_leq lexn1 observer.
+    + (* in this case all exceptions are visible, with this constraint everything is 
+         is fine, because visible exceptions must match up on both sides *) admit.
+    + (* in this case there might be invisble exceptions 
+         but maybe the pc somehow saved us from making any mistakes
+       *)
+    specialize (Hc2 observer). inv Hc2.
+Abort.
+          
+(* I'm actually a bit confused as to why this went through so easily 
+   why don't I need to do case analysis on whether exceptions are output?
+ *)
+(* Today, 
+
+
+  1: work out definition for exception part of legical relation
+  2: work out Seq case
+
+*)
